dsub.v: Finish adapting stlc.v to bigger language

ecoop17/dsub.v
@@ -493,254 +493,279 @@ Definition wk n' := rename (fun n => n + n').
 
 (* Adapted from dot_eval.v *)
 
-(* Fixpoint tevalSM (t: tm) (n: nat) (env: venv): option (option vl * nat) := *)
-(*   match n with *)
-(*   | 0 => None *)
-(*   | S n => *)
-(*     match t with *)
-(*     | tvar x       => ret (indexr x env, 0) *)
-(*     (* | ttyp T       => ret (vty env T) *) *)
-(*     | tabs y     => ret (vabs env y) *)
-(*     | trec y     => ret (vrec env y) *)
-(*     | tnat n     => ret (vnat n) *)
-(*     | tapp tf ta   => *)
-(*       va <- tevalSM ta n env; *)
-(*       vf <- tevalSM tf n env; *)
-(*       match vf with *)
-(*       | vabs env2 tbody => *)
-(*         tevalSM tbody n (va :: env2) *)
-(*       | vrec env2 tbody => *)
-(*         logStep 1 (tevalSM tbody n (va :: vf :: env2)) *)
-(*       | _ => error *)
-(*       end *)
-(*     | tlet t1 t2 => *)
-(*       v1 <- tevalSM t1 n env; *)
-(*       (* Omit counting an extra step, since this let is not recursive! *) *)
-(*       tevalSM t2 n (v1 :: env) *)
-(*     (* | tunpack tx ty => *) *)
-(*     (*   vx <- tevalSM tx n env; *) *)
-(*     (*   logStep 1 (tevalSM ty n (vx::env)) *) *)
-(*     end *)
-(*   end. *)
+Fixpoint tevalSM (t: tm) (n: nat) (env: venv): option (option vl * nat) :=
+  match n with
+  | 0 => None
+  | S n =>
+    match t with
+    | tvar x       => ret (indexr x env, 0)
+    (* | ttyp T       => ret (vty env T) *)
+    | tabs y     => ret (vabs env y)
+    | trec y     => ret (vrec env y)
+    | tnat n     => ret (vnat n)
+    | tpack T t =>
+      v <- tevalSM t n env;
+      ret (vpack env T v)
+    | tproj t =>
+      v <- tevalSM t n env;
+      match v with
+      | vpack env T v => ret v
+      | _ => error
+      end
+    | tapp tf ta   =>
+      va <- tevalSM ta n env;
+      vf <- tevalSM tf n env;
+      match vf with
+      | vabs env2 tbody =>
+        tevalSM tbody n (va :: env2)
+      | vrec env2 tbody =>
+        logStep 1 (tevalSM tbody n (va :: vf :: env2))
+      | _ => error
+      end
+    | tlet t1 t2 =>
+      v1 <- tevalSM t1 n env;
+      (* Omit counting an extra step, since this let is not recursive! *)
+      tevalSM t2 n (v1 :: env)
+    (* | tunpack tx ty => *)
+    (*   vx <- tevalSM tx n env; *)
+    (*   logStep 1 (tevalSM ty n (vx::env)) *)
+    end
+  end.
 
-(* Fixpoint tevalS (t: tm) (n: nat) (env: venv): option (option vl * nat) := *)
-(*   match n with *)
-(*     | 0 => None *)
-(*     | S n => *)
-(*       match t with *)
-(*         | tvar x       => Some (indexr x env, 0) *)
-(*         (* | ttyp T       => Some (Some (vty env T), 0) *) *)
-(*         | tabs y     => Some (Some (vabs env y), 0) *)
-(*         | trec y     => Some (Some (vrec env y), 0) *)
-(*         | tnat n     => Some (Some (vnat n), 0) *)
-(*         | tapp ef ex   => *)
-(*           match tevalS ex n env with *)
-(*             | None => None *)
-(*             | Some (None, k1) => Some (None, k1) *)
-(*             | Some (Some vx, k1) => *)
-(*               match tevalS ef n env with *)
-(*                 | None => None *)
-(*                 | Some (None, k2) => Some (None, k1 + k2) *)
-(*                 | Some (Some vf, k2) => *)
-(*                   match vf with *)
-(*                   | vabs env2 ey => logStep (k1 + k2) (tevalS ey n (vx::env2)) *)
-(*                   | vrec env2 ey => logStep (k1 + k2 + 1) (tevalS ey n (vx::vf::env2)) *)
-(*                   | _ => Some (None, k1 + k2) *)
-(*                   end *)
-(*               end *)
-(*           end *)
-(*         | tlet e1 e2 => *)
-(*           match tevalS e1 n env with *)
-(*           | None => None *)
-(*           | Some (None, k1) => Some (None, k1) *)
-(*           | Some (Some v1, k1) => *)
-(*             (* logStep (k1 + 1) *) *)
-(*             logStep k1 (tevalS e2 n (v1 :: env)) *)
-(*           end *)
+Fixpoint tevalS (t: tm) (n: nat) (env: venv): option (option vl * nat) :=
+  match n with
+    | 0 => None
+    | S n =>
+      match t with
+        | tvar x       => Some (indexr x env, 0)
+        (* | ttyp T       => Some (Some (vty env T), 0) *)
+        | tabs y     => Some (Some (vabs env y), 0)
+        | trec y     => Some (Some (vrec env y), 0)
+        | tnat n     => Some (Some (vnat n), 0)
+        | tpack T t =>
+          match (tevalS t n env) with
+          | None => None
+          | Some (None, k1) => Some (None, k1)
+          | Some (Some v, k1) => Some (Some (vpack env T v), k1)
+          end
+        | tproj t =>
+          match (tevalS t n env) with
+          | None => None
+          | Some (None, k1) => Some (None, k1)
+          | Some (Some v, k1) =>
+            match v with 
+            | vpack env T v => Some (Some v, k1)
+            | _ => Some (None, k1)
+            end
+          end
+        | tapp ef ex   =>
+          match tevalS ex n env with
+            | None => None
+            | Some (None, k1) => Some (None, k1)
+            | Some (Some vx, k1) =>
+              match tevalS ef n env with
+                | None => None
+                | Some (None, k2) => Some (None, k1 + k2)
+                | Some (Some vf, k2) =>
+                  match vf with
+                  | vabs env2 ey => logStep (k1 + k2) (tevalS ey n (vx::env2))
+                  | vrec env2 ey => logStep (k1 + k2 + 1) (tevalS ey n (vx::vf::env2))
+                  | _ => Some (None, k1 + k2)
+                  end
+              end
+          end
+        | tlet e1 e2 =>
+          match tevalS e1 n env with
+          | None => None
+          | Some (None, k1) => Some (None, k1)
+          | Some (Some v1, k1) =>
+            (* logStep (k1 + 1) *)
+            logStep k1 (tevalS e2 n (v1 :: env))
+          end
 
-(*         (* | tunpack ex ey => *) *)
-(*         (*   match tevalS ex n env with *) *)
-(*         (*     | None => None *) *)
-(*         (*     | Some (None, k) => Some (None, k) *) *)
-(*         (*     | Some (Some vx, k1) => *) *)
-(*         (*       logStep (k1 + 1) (tevalS ey n (vx::env)) *) *)
-(*         (*   end *) *)
-(*       end *)
-(*   end. *)
+        (* | tunpack ex ey => *)
+        (*   match tevalS ex n env with *)
+        (*     | None => None *)
+        (*     | Some (None, k) => Some (None, k) *)
+        (*     | Some (Some vx, k1) => *)
+        (*       logStep (k1 + 1) (tevalS ey n (vx::env)) *)
+        (*   end *)
+      end
+  end.
 
-(* Theorem evalMs_equiv: forall n env t, tevalSM t n env = tevalS t n env. *)
-(* Proof. *)
-(*   intros; revert env t; induction n; simpl_unfold_monad; unfold logStep; try reflexivity; *)
-(*     intros; *)
-(*     repeat progress *)
-(*       (try better_case_match_ex; *)
-(*        repeat fequalSafe; *)
-(*        repeat rewrite IHn in *; *)
-(*        try abstract (reflexivity || discriminate || omega)). *)
-(* Qed. *)
-(* (** Define "evaluation with enough fuel". *)
+Theorem evalMs_equiv: forall n env t, tevalSM t n env = tevalS t n env.
+Proof.
+  intros; revert env t; induction n; simpl_unfold_monad; unfold logStep; try reflexivity;
+    intros;
+    repeat progress
+      (try better_case_match_ex;
+       repeat fequalSafe;
+       repeat rewrite IHn in *;
+       try abstract (reflexivity || discriminate || omega)).
+Qed.
+(** Define "evaluation with enough fuel". *)
 (*     We can show that adding more fuel to evaluation that doesn't time out gives *)
 (*     the same result. But we can also build that in our assumptions. *)
-(*  *) *)
-(* Definition tevalSnmOpt env e optV k nm := forall n, n > nm -> tevalS e n env = Some (optV, k). *)
-(* Definition tevalSnm env e v k nm := tevalSnmOpt env e (Some v) k nm. *)
-(* Definition tevalSnOpt env e optV k := exists nm, tevalSnmOpt env e optV k nm. *)
-(* Definition tevalSn env e v k := tevalSnOpt env e (Some v) k. *)
+(*  *)
+Definition tevalSnmOpt env e optV k nm := forall n, n > nm -> tevalS e n env = Some (optV, k).
+Definition tevalSnm env e v k nm := tevalSnmOpt env e (Some v) k nm.
+Definition tevalSnOpt env e optV k := exists nm, tevalSnmOpt env e optV k nm.
+Definition tevalSn env e v k := tevalSnOpt env e (Some v) k.
 
-(* Hint Transparent tevalSnOpt tevalSnm tevalSn. *)
-(* Ltac unfold2tevalSnmOpt := unfold tevalSn, tevalSnOpt, tevalSnm in *. *)
-(* Ltac unfoldTeval := unfold2tevalSnmOpt; unfold tevalSnmOpt in *. *)
+Hint Transparent tevalSnOpt tevalSnm tevalSn.
+Ltac unfold2tevalSnmOpt := unfold tevalSn, tevalSnOpt, tevalSnm in *.
+Ltac unfoldTeval := unfold2tevalSnmOpt; unfold tevalSnmOpt in *.
 
-(* Ltac n_is_succ_hp := *)
-(*   ev; match goal with *)
-(*   | H : forall n, n > ?nm -> _ |- _ => *)
-(*     let H2 := fresh "H" in *)
-(*     lets ? : H (S nm) __; eauto; clear H; simpl in H2; try unfold logStep in H2 *)
-(*   end. *)
+Ltac n_is_succ_hp :=
+  ev; match goal with
+  | H : forall n, n > ?nm -> _ |- _ =>
+    let H2 := fresh "H" in
+    lets ? : H (S nm) __; eauto; clear H; simpl in H2; try unfold logStep in H2
+  end.
 
-(* (** [tevalSnmOpt] (expanded) is monotonic relative to [nm]. This does not *)
-(*     follow from properties of [tevalS], but by construction of [tevalSnmOpt]. *) *)
-(* Lemma tevalS_kripke_mono: forall env e optV k nm1, *)
-(*     (forall n, n > nm1 -> tevalS e n env = Some (optV, k)) -> *)
-(*     forall nm2, nm2 >= nm1 -> *)
-(*     forall n, n > nm2 -> tevalS e n env = Some (optV, k). *)
-(* Proof. eauto. Qed. *)
-(* Hint Resolve tevalS_kripke_mono. *)
+(** [tevalSnmOpt] (expanded) is monotonic relative to [nm]. This does not *)
+(*     follow from properties of [tevalS], but by construction of [tevalSnmOpt]. *)
+Lemma tevalS_kripke_mono: forall env e optV k nm1,
+    (forall n, n > nm1 -> tevalS e n env = Some (optV, k)) ->
+    forall nm2, nm2 >= nm1 ->
+    forall n, n > nm2 -> tevalS e n env = Some (optV, k).
+Proof. eauto. Qed.
+Hint Resolve tevalS_kripke_mono.
 
-(* (** [tevalSnmOpt] is monotonic relative to [nm]. This does not follow from *)
-(*     properties of [tevalS], but by construction of [tevalSnmOpt]. *) *)
-(* Lemma tevalSnmOpt_mono: forall env e optV k nm1, *)
-(*     tevalSnmOpt env e optV k nm1 -> *)
-(*     forall nm2, nm2 >= nm1 -> *)
-(*     tevalSnmOpt env e optV k nm2. *)
-(* Proof. intros; unfoldTeval; eauto using tevalS_kripke_mono. Qed. *)
+(** [tevalSnmOpt] is monotonic relative to [nm]. This does not follow from *)
+(*     properties of [tevalS], but by construction of [tevalSnmOpt]. *)
+Lemma tevalSnmOpt_mono: forall env e optV k nm1,
+    tevalSnmOpt env e optV k nm1 ->
+    forall nm2, nm2 >= nm1 ->
+    tevalSnmOpt env e optV k nm2.
+Proof. intros; unfoldTeval; eauto using tevalS_kripke_mono. Qed.
 
-(* Lemma max_bigger_both: forall n1 n2, max n1 n2 >= n1 /\ max n1 n2 >= n2. *)
-(*   intuition eauto using Nat.le_max_l, Nat.le_max_r. *)
-(* Qed. *)
+Lemma max_bigger_both: forall n1 n2, max n1 n2 >= n1 /\ max n1 n2 >= n2.
+  intuition eauto using Nat.le_max_l, Nat.le_max_r.
+Qed.
 
-(* Ltac alignTevalAssumptions := *)
-(*   unfoldTeval; *)
-(*   match goal with *)
-(*   | H1 : forall n, n > ?nm1 -> tevalS ?t n ?env = Some ?t1 , H2 : forall n, n > ?nm2 -> tevalS ?t n ?env = Some ?t2 |- _ => *)
-(*     let nm := fresh "nm" in *)
-(*     remember (max (nm1) (nm2)) as nm; *)
-(*     assert (nm >= nm1 /\ nm >= nm2) as (? & ?) by (subst; eauto using max_bigger_both); *)
-(*     assert (tevalSnmOpt env t (fst t1) (snd t1) nm) by (simpl; unfoldTeval; eauto); *)
-(*     assert (tevalSnmOpt env t (fst t2) (snd t2) nm) by (simpl; unfoldTeval; eauto); *)
-(*     clear H1 H2; *)
-(*     unfoldTeval *)
-(*   end. *)
+Ltac alignTevalAssumptions :=
+  unfoldTeval;
+  match goal with
+  | H1 : forall n, n > ?nm1 -> tevalS ?t n ?env = Some ?t1 , H2 : forall n, n > ?nm2 -> tevalS ?t n ?env = Some ?t2 |- _ =>
+    let nm := fresh "nm" in
+    remember (max (nm1) (nm2)) as nm;
+    assert (nm >= nm1 /\ nm >= nm2) as (? & ?) by (subst; eauto using max_bigger_both);
+    assert (tevalSnmOpt env t (fst t1) (snd t1) nm) by (simpl; unfoldTeval; eauto);
+    assert (tevalSnmOpt env t (fst t2) (snd t2) nm) by (simpl; unfoldTeval; eauto);
+    clear H1 H2;
+    unfoldTeval
+  end.
 
-(* Lemma tevalS_det: forall optV1 optV2 env t j1 j2 nm1 nm2, *)
-(*   (forall n : nat, n > nm1 -> tevalS t n env = Some (optV1, j1)) -> *)
-(*   (forall n : nat, n > nm2 -> tevalS t n env = Some (optV2, j2)) -> *)
-(*   optV1 = optV2 /\ j1 = j2. *)
-(* Proof. *)
-(*   intros; alignTevalAssumptions; *)
-(*     repeat n_is_succ_hp; optFuncs_det; eauto. *)
-(* Qed. *)
+Lemma tevalS_det: forall optV1 optV2 env t j1 j2 nm1 nm2,
+  (forall n : nat, n > nm1 -> tevalS t n env = Some (optV1, j1)) ->
+  (forall n : nat, n > nm2 -> tevalS t n env = Some (optV2, j2)) ->
+  optV1 = optV2 /\ j1 = j2.
+Proof.
+  intros; alignTevalAssumptions;
+    repeat n_is_succ_hp; optFuncs_det; eauto.
+Qed.
 
-(* (* Experiment on different way of writing tevalS_det: can we make auto happier about injecting p1 = p2 than splitting it? *) *)
-(* Lemma tevalS_det2: forall optV1 optV2 env t j1 j2 nm1 nm2, *)
-(*   (forall n : nat, n > nm1 -> tevalS t n env = Some (optV1, j1)) -> *)
-(*   (forall n : nat, n > nm2 -> tevalS t n env = Some (optV2, j2)) -> *)
-(*   (optV1, j1) = (optV2, j2). *)
-(* Proof. *)
-(*   intros; alignTevalAssumptions; *)
-(*     repeat n_is_succ_hp; optFuncs_det; eauto. *)
-(* Qed. *)
+(* Experiment on different way of writing tevalS_det: can we make auto happier about injecting p1 = p2 than splitting it? *)
+Lemma tevalS_det2: forall optV1 optV2 env t j1 j2 nm1 nm2,
+  (forall n : nat, n > nm1 -> tevalS t n env = Some (optV1, j1)) ->
+  (forall n : nat, n > nm2 -> tevalS t n env = Some (optV2, j2)) ->
+  (optV1, j1) = (optV2, j2).
+Proof.
+  intros; alignTevalAssumptions;
+    repeat n_is_succ_hp; optFuncs_det; eauto.
+Qed.
 
-(* Tactic Notation "try_once_tac" constr(T) tactic(tac) := *)
-(*   match goal with *)
-(*   | H : usedLemma T |- _ => fail 1 *)
-(*   | _ => markUsed T; tac *)
-(*   end. *)
+Tactic Notation "try_once_tac" constr(T) tactic(tac) :=
+  match goal with
+  | H : usedLemma T |- _ => fail 1
+  | _ => markUsed T; tac
+  end.
 
-(* Definition injectHyps_marker := 0. *)
-(* Hint Extern 5 => try_once_tac injectHyps_marker injectHyps. *)
-(* (* Hint Extern 5 => optFuncs_det. *) *)
+Definition injectHyps_marker := 0.
+Hint Extern 5 => try_once_tac injectHyps_marker injectHyps.
+(* Hint Extern 5 => optFuncs_det. *)
 
-(* (* XXX this used tevalS_detp, the next uses _det, seems _detp might not be that useful here yet... *) *)
-(* Lemma tevalS_det_optV: forall optV1 optV2 env t j1 j2 nm1 nm2, *)
-(*   (forall n : nat, n > nm1 -> tevalS t n env = Some (optV1, j1)) -> *)
-(*   (forall n : nat, n > nm2 -> tevalS t n env = Some (optV2, j2)) -> *)
-(*   optV1 = optV2. *)
-(* Proof. intros. lets ?: tevalS_det2 optV1 optV2 ___; eauto. Qed. *)
+(* XXX this used tevalS_detp, the next uses _det, seems _detp might not be that useful here yet... *)
+Lemma tevalS_det_optV: forall optV1 optV2 env t j1 j2 nm1 nm2,
+  (forall n : nat, n > nm1 -> tevalS t n env = Some (optV1, j1)) ->
+  (forall n : nat, n > nm2 -> tevalS t n env = Some (optV2, j2)) ->
+  optV1 = optV2.
+Proof. intros. lets ?: tevalS_det2 optV1 optV2 ___; eauto. Qed.
 
-(* (* Hint Extern 5 => ev. *) *)
+(* Hint Extern 5 => ev. *)
 
-(* Lemma tevalS_det_j: forall optV1 optV2 env t j1 j2 nm1 nm2, *)
-(*   (forall n : nat, n > nm1 -> tevalS t n env = Some (optV1, j1)) -> *)
-(*   (forall n : nat, n > nm2 -> tevalS t n env = Some (optV2, j2)) -> *)
-(*   j1 = j2. *)
-(* Proof. intros; lets ?: tevalS_det optV1 optV2 ___; ev; eauto. Qed. *)
+Lemma tevalS_det_j: forall optV1 optV2 env t j1 j2 nm1 nm2,
+  (forall n : nat, n > nm1 -> tevalS t n env = Some (optV1, j1)) ->
+  (forall n : nat, n > nm2 -> tevalS t n env = Some (optV2, j2)) ->
+  j1 = j2.
+Proof. intros; lets ?: tevalS_det optV1 optV2 ___; ev; eauto. Qed.
 
-(* Hint Resolve tevalS_det_optV tevalS_det_j. *)
+Hint Resolve tevalS_det_optV tevalS_det_j.
 
-(* Lemma tevalSnmOpt_det_optV: forall env t optV1 optV2 j1 j2 nm1 nm2, *)
-(*     tevalSnmOpt env t optV1 j1 nm1 -> *)
-(*     tevalSnmOpt env t optV2 j2 nm2 -> *)
-(*     optV1 = optV2. *)
-(* Proof. (* firstorder eauto. (* Or: *) *) intros; unfoldTeval; eauto. Qed. *)
+Lemma tevalSnmOpt_det_optV: forall env t optV1 optV2 j1 j2 nm1 nm2,
+    tevalSnmOpt env t optV1 j1 nm1 ->
+    tevalSnmOpt env t optV2 j2 nm2 ->
+    optV1 = optV2.
+Proof. (* firstorder eauto. (* Or: *) *) intros; unfoldTeval; eauto. Qed.
 
-(* Lemma tevalSnmOpt_det_j: forall env t optV1 optV2 j1 j2 nm1 nm2, *)
-(*     tevalSnmOpt env t optV1 j1 nm1 -> *)
-(*     tevalSnmOpt env t optV2 j2 nm2 -> *)
-(*     j1 = j2. *)
-(* Proof. unfoldTeval; eauto. Qed. *)
+Lemma tevalSnmOpt_det_j: forall env t optV1 optV2 j1 j2 nm1 nm2,
+    tevalSnmOpt env t optV1 j1 nm1 ->
+    tevalSnmOpt env t optV2 j2 nm2 ->
+    j1 = j2.
+Proof. unfoldTeval; eauto. Qed.
 
-(* Hint Resolve tevalSnmOpt_det_optV tevalSnmOpt_det_j. *)
+Hint Resolve tevalSnmOpt_det_optV tevalSnmOpt_det_j.
 
-(* Lemma tevalSnmOpt_det: forall env t optV1 optV2 j1 j2 nm1 nm2, *)
-(*     tevalSnmOpt env t optV1 j1 nm1 -> *)
-(*     tevalSnmOpt env t optV2 j2 nm2 -> *)
-(*     optV1 = optV2 /\ j1 = j2. *)
-(* Proof. eauto. Qed. *)
+Lemma tevalSnmOpt_det: forall env t optV1 optV2 j1 j2 nm1 nm2,
+    tevalSnmOpt env t optV1 j1 nm1 ->
+    tevalSnmOpt env t optV2 j2 nm2 ->
+    optV1 = optV2 /\ j1 = j2.
+Proof. eauto. Qed.
 
-(* (* Convince Coq that if n > m then n = S n' for some n', then there's enough *)
-(*    fuel to perform one evaluation step. *) *)
-(* Lemma n_to_Sn: forall n m, n > m -> exists n', n = S n'. *)
-(*   intros; destruct n; [ exfalso; omega | eauto]. *)
-(* Qed. *)
-(* Hint Unfold gt ge lt. *)
-(* Hint Transparent gt ge lt. *)
+(* Convince Coq that if n > m then n = S n' for some n', then there's enough *)
+(*    fuel to perform one evaluation step. *)
+Lemma n_to_Sn: forall n m, n > m -> exists n', n = S n'.
+  intros; destruct n; [ exfalso; omega | eauto].
+Qed.
+Hint Unfold gt ge lt.
+Hint Transparent gt ge lt.
 
-(* Tactic Notation "n_is_succ'" simple_intropattern(P) := *)
-(*   unfold gt, ge, lt in *; *)
-(*   match goal with *)
-(*   | [H : S ?m <= ?n |- _] => lets [P ->]: n_to_Sn H *)
-(*   end. *)
+Tactic Notation "n_is_succ'" simple_intropattern(P) :=
+  unfold gt, ge, lt in *;
+  match goal with
+  | [H : S ?m <= ?n |- _] => lets [P ->]: n_to_Sn H
+  end.
 
-(* Ltac n_is_succ := let n' := fresh "n" in n_is_succ' n'. *)
+Ltac n_is_succ := let n' := fresh "n" in n_is_succ' n'.
 
-(* Ltac step_eval := n_is_succ; simpl in *. *)
-(* (* Hint Extern 5 => step_eval. *) *)
+Ltac step_eval := n_is_succ; simpl in *.
+(* Hint Extern 5 => step_eval. *)
 
-(* Lemma inv_tevalS: forall t n env r, tevalS t n env = Some r -> exists n', n = S n'. *)
-(* Proof. intros; destruct n; discriminate || eauto. Qed. *)
+Lemma inv_tevalS: forall t n env r, tevalS t n env = Some r -> exists n', n = S n'.
+Proof. intros; destruct n; discriminate || eauto. Qed.
 
-(* Ltac inv_tevalS := *)
-(*   lazymatch goal with *)
-(*   | H : tevalS _ ?n _ = Some _ |- _ => *)
-(*     let n' := fresh n in *)
-(*     lets (n' & ->) : inv_tevalS H *)
-(*   end. *)
+Ltac inv_tevalS :=
+  lazymatch goal with
+  | H : tevalS _ ?n _ = Some _ |- _ =>
+    let n' := fresh n in
+    lets (n' & ->) : inv_tevalS H
+  end.
 
 
-(* Lemma teval_var: forall env x, *)
-(*   exists optV, tevalSnOpt env (tvar x) optV 0 /\ indexr x env = optV. *)
-(* Proof. unfoldTeval; eexists; split_conj; try exists 0; intros; try step_eval; trivial. Qed. *)
-(* Hint Resolve teval_var. *)
+Lemma teval_var: forall env x,
+  exists optV, tevalSnOpt env (tvar x) optV 0 /\ indexr x env = optV.
+Proof. unfoldTeval; eexists; split_conj; try exists 0; intros; try step_eval; trivial. Qed.
+Hint Resolve teval_var.
 
-(* Ltac eval_det := *)
-(*   unfold2tevalSnmOpt; ev; *)
-(*   match goal with *)
-(*   | H1 : tevalSnmOpt _ _ _ _ _, H2 : tevalSnmOpt _ _ _ _ _ |- _ => *)
-(*     lets (? & ?) : tevalSnmOpt_det H1 H2 ___ *)
-(*   end; injectHyps. *)
+Ltac eval_det :=
+  unfold2tevalSnmOpt; ev;
+  match goal with
+  | H1 : tevalSnmOpt _ _ _ _ _, H2 : tevalSnmOpt _ _ _ _ _ |- _ =>
+    lets (? & ?) : tevalSnmOpt_det H1 H2 ___
+  end; injectHyps.
 
-(* (** Fuel monotonicity: If evaluation does not time out, increasing fuel preserves the result. *)
+(** Fuel monotonicity: If evaluation does not time out, increasing fuel preserves the result. *)
 (*  **** Proof sketch. *)
 (*       By induction on the available fuel [n] in the initial evaluation and case *)
 (*       analysis on terms. *)
@@ -749,114 +774,114 @@ Definition wk n' := rename (fun n => n + n').
 (*       the induction hypothesis they satisfy fuel monotonicity, the recursive *)
 (*       calls with more fuel give the same result, hence overall evaluation with *)
 (*       more fuel gives the same result. *)
-(*  *) *)
-(* Lemma tevalS_mono: forall n e env optV, tevalS e n env = Some optV -> forall m, m >= n -> tevalS e m env = Some optV. *)
-(* Proof. *)
-(*   (** [tevalS_det] applies the induction hypothesis to recursive calls. *) *)
-(*   Ltac tevalS_det n m' IHn := *)
-(*     match goal with *)
-(*     | H1: tevalS ?e n ?env = Some ?r1, H2 : tevalS ?e m' ?env = ?r2 |- _ => *)
-(*       let H := fresh "H" in *)
-(*       assert (tevalS e m' env = Some r1) as H by (eapply IHn; auto 1); *)
-(*       rewrite H in *; clear H *)
-(*     end. *)
+(*  *)
+Lemma tevalS_mono: forall n e env optV, tevalS e n env = Some optV -> forall m, m >= n -> tevalS e m env = Some optV.
+Proof.
+  (** [tevalS_det] applies the induction hypothesis to recursive calls. *)
+  Ltac tevalS_det n m' IHn :=
+    lazymatch goal with
+    | H1: tevalS ?e n ?env = Some ?r1, H2 : tevalS ?e m' ?env = ?r2 |- _ =>
+      let H := fresh "H" in
+      assert (tevalS e m' env = Some r1) as H by (eapply IHn; auto 1);
+      rewrite H in *; clear H
+    end.
 
-(*   induction n; intros * Heval * Hmn; try solve [inverse Heval]; *)
-(*   n_is_succ' m'; *)
+  induction n; intros * Heval * Hmn; try solve [inverse Heval];
+  n_is_succ' m';
 
-(*   generalize dependent optV; generalize dependent n; destruct e; *)
-(*     intros; simpl in *; unfold logStep in *; *)
-(*     trivial; *)
+  generalize dependent optV; generalize dependent n; destruct e;
+    intros; simpl in *; unfold logStep in *;
+    trivial;
 
-(*   repeat (better_case_match_ex; try tevalS_det n m' IHn); trivial. *)
-(* Qed. *)
-(* Hint Resolve tevalS_mono. *)
+  repeat (better_case_match_ex; subst; try tevalS_det n m' IHn); trivial.
+Qed.
+Hint Resolve tevalS_mono.
 
-(* (**********************) *)
-(* (** Logical relation. *) *)
+(**********************)
+(** Logical relation. *)
 
-(* Require Import Coq.Relations.Relation_Operators. *)
-(* (* Require Export Coq.Wellfounded.Lexicographic_Product. *) *)
+Require Import Coq.Relations.Relation_Operators.
+(* Require Export Coq.Wellfounded.Lexicographic_Product. *)
 
-(* (*******************) *)
-(* (* Define language infrastructure. *) *)
+(*******************)
+(* Define language infrastructure. *)
 
-(* Definition vl_prop := vl -> Prop. *)
-(* Hint Unfold vl_prop. *)
+Definition vl_prop := vl -> Prop.
+Hint Unfold vl_prop.
 
-(* Module Type vtp_arg. *)
-(*   Parameter vtp : ty -> vl_prop. *)
-(*   Parameter expr_sem : vl_prop -> tm -> venv -> Prop. *)
-(* End vtp_arg. *)
+Module Type vtp_arg.
+  Parameter vtp : ty -> vl_prop.
+  Parameter expr_sem : vl_prop -> tm -> venv -> Prop.
+End vtp_arg.
 
-(* Module Envs (VTP: vtp_arg). *)
-(*   Import VTP. *)
+Module Envs (VTP: vtp_arg).
+  Import VTP.
 
-(*   (* Copy-pasted and modularizable. *) *)
-(*   Inductive R_env : venv -> tenv -> Set := *)
-(*   | R_nil : *)
-(*       R_env [] [] *)
-(*   | R_cons : forall T v env G, *)
-(*       R_env env G -> *)
-(*       vtp T v -> *)
-(*       R_env (v :: env) (T :: G). *)
-(*   Hint Constructors R_env. *)
+  (* Copy-pasted and modularizable. *)
+  Inductive R_env : venv -> tenv -> Set :=
+  | R_nil :
+      R_env [] []
+  | R_cons : forall T v env G,
+      R_env env G ->
+      vtp T v ->
+      R_env (v :: env) (T :: G).
+  Hint Constructors R_env.
 
-(*   Lemma wf_length : forall vs ts, *)
-(*       R_env vs ts -> *)
-(*       (length vs = length ts). *)
-(*   Proof. intros * H; induction H; simpl; congruence. Qed. *)
+  Lemma wf_length : forall vs ts,
+      R_env vs ts ->
+      (length vs = length ts).
+  Proof. intros * H; induction H; simpl; congruence. Qed.
 
-(*   Ltac lenG_to_lenEnv := *)
-(*     try match goal with *)
-(*         | H: R_env ?env ?G |- _ => *)
-(*           replace (length G) with (length env) in * by (eauto using wf_length) *)
-(*         end. *)
+  Ltac lenG_to_lenEnv :=
+    try match goal with
+        | H: R_env ?env ?G |- _ =>
+          replace (length G) with (length env) in * by (eauto using wf_length)
+        end.
 
-(*   Lemma R_env_to_indexr_success: forall G env x T, indexr x G = Some T -> R_env env G -> exists v, indexr x env = Some v. *)
-(*     intros * HT Henv; induction Henv; simpl in *; *)
-(*       tryfalse; *)
-(*       lenG_to_lenEnv; better_case_match_ex; eauto. *)
-(*   Qed. *)
-(*   Hint Resolve R_env_to_indexr_success. *)
+  Lemma R_env_to_indexr_success: forall G env x T, indexr x G = Some T -> R_env env G -> exists v, indexr x env = Some v.
+    intros * HT Henv; induction Henv; simpl in *;
+      tryfalse;
+      lenG_to_lenEnv; better_case_match_ex; eauto.
+  Qed.
+  Hint Resolve R_env_to_indexr_success.
 
-(*   Lemma R_env_to_vtp: forall G env x T v, indexr x G = Some T -> indexr x env = Some v -> R_env env G -> vtp T v. *)
-(*   Proof. *)
-(*     intros * HT Hv Henv; induction Henv; simpl in *; *)
-(*       [ discriminate | *)
-(*         lenG_to_lenEnv; *)
-(*         repeat (better_case_match; beq_nat); eauto]. *)
-(*   Qed. *)
-(*   Hint Resolve R_env_to_vtp. *)
-(*   (* Copy-pasted and modularizable, until at least here. *) *)
+  Lemma R_env_to_vtp: forall G env x T v, indexr x G = Some T -> indexr x env = Some v -> R_env env G -> vtp T v.
+  Proof.
+    intros * HT Hv Henv; induction Henv; simpl in *;
+      [ discriminate |
+        lenG_to_lenEnv;
+        repeat (better_case_match; beq_nat); eauto].
+  Qed.
+  Hint Resolve R_env_to_vtp.
+  (* Copy-pasted and modularizable, until at least here. *)
 
-(*   Definition etp T e env := *)
-(*     expr_sem (fun v => vtp T v) e env. *)
+  Definition etp T e env :=
+    expr_sem (fun v => vtp T v) e env.
 
-(*   (* Semantic typing *) *)
-(*   Definition sem_type (G : tenv) (T : ty) (e: tm) := *)
-(*     forall env, *)
-(*       R_env env G -> *)
-(*       etp T e env. *)
+  (* Semantic typing *)
+  Definition sem_type (G : tenv) (T : ty) (e: tm) :=
+    forall env,
+      R_env env G ->
+      etp T e env.
 
-(*   Definition sem_vl_subtype (G : tenv) (T1 T2: ty) := *)
-(*     (* wf G T1 /\ *) *)
-(*     (* wf G T2 /\ *) *)
-(*     (* forall env, *) *)
-(*     (*   R_env env G -> *) *)
-(*     forall v, vtp T1 v -> vtp T2 v. *)
+  Definition sem_vl_subtype (G : tenv) (T1 T2: ty) :=
+    (* wf G T1 /\ *)
+    (* wf G T2 /\ *)
+    (* forall env, *)
+    (*   R_env env G -> *)
+    forall v, vtp T1 v -> vtp T2 v.
 
-(*   Definition sem_subtype (G : tenv) (T1 T2: ty) := *)
-(*     (* wf G T1 /\ *) *)
-(*     (* wf G T2 /\ *) *)
-(*     sem_vl_subtype G T1 T2 /\ *)
-(*     forall env, *)
-(*       R_env env G -> *)
-(*       forall e, etp T1 e env -> etp T2 e env. *)
+  Definition sem_subtype (G : tenv) (T1 T2: ty) :=
+    (* wf G T1 /\ *)
+    (* wf G T2 /\ *)
+    sem_vl_subtype G T1 T2 /\
+    forall env,
+      R_env env G ->
+      forall e, etp T1 e env -> etp T2 e env.
 
-(*   Lemma subtype_to_vl_subtype : forall G T1 T2, *)
-(*       sem_subtype G T1 T2 -> sem_vl_subtype G T1 T2. *)
-(*   Proof. unfold sem_subtype; tauto. Qed. *)
-(*   Hint Resolve subtype_to_vl_subtype. *)
+  Lemma subtype_to_vl_subtype : forall G T1 T2,
+      sem_subtype G T1 T2 -> sem_vl_subtype G T1 T2.
+  Proof. unfold sem_subtype; tauto. Qed.
+  Hint Resolve subtype_to_vl_subtype.
 
-(* End Envs. *)
+End Envs.
